commit

Projects/Esolangs/Cornucopia/Basic.lean
@@ -2,56 +2,901 @@ import Projects.Esolangs.Cornucopia.Defs
 
 attribute [-simp] List.getElem!_eq_getElem?_getD
 
+section logic
+
+@[simp] theorem or_iff_or_left {p q r : Prop} : (p ∨ q ↔ p ∨ r) ↔ ¬p → (q ↔ r) := by tauto
+@[simp] theorem or_iff_or_right {p q r : Prop} : (p ∨ q ↔ r ∨ q) ↔ ¬q → (p ↔ r) := by tauto
+@[simp] theorem imp_not_imp_iff {p q : Prop} : p → ¬p → q ↔ True := by tauto
+@[simp] theorem not_imp_imp_iff {p q : Prop} : ¬p → p → q ↔ True := by tauto
+
+-- #check 0 #exit
+
+end logic
+
+namespace List
+
+variable {α β γ : Type*}
+variable {xs ys zs : List α}
+
+@[simp]
+theorem length_mkList {n} {f : ℕ → α} : (mkList n f).length = n := by
+  simp [mkList]
+
+@[simp]
+theorem mem_mkList {n} {f : ℕ → α} {x} : x ∈ mkList n f ↔ ∃ i < n, f i = x := by
+  simp [mkList]
+
+theorem mergeSort_eq_mergeSort_iff {le : α → α → Bool}
+(trans : ∀ (a b c : α), le a b → le b c → le a c)
+(total : ∀ (a b : α), le a b || le b a)
+(antisymm : ∀ (a b : α), le a b → le b a → a = b) :
+xs.mergeSort le = ys.mergeSort le ↔ xs.Perm ys := by
+  use perm_of_mergeSort_eq_mergeSort
+  intro h
+  apply eq_of_perm_of_pairwise (r := (le · ·))
+  · simpa
+  · apply pairwise_mergeSort trans total
+  · apply pairwise_mergeSort trans total
+  · grind
+  · grind
+  · grind
+
+@[simp]
+theorem map_mkList {n} {f : ℕ → α} {g : α → β} :
+(mkList n f).map g = mkList n λ i => g (f i) := by
+  simp [mkList]
+
+@[simp]
+theorem getElem_mkList {n} {f : ℕ → α} {i}
+{h : i < (mkList n f).length} : (mkList n f)[i] = f i := by
+  simp [mkList]
+
+@[simp]
+theorem mkList_length_getElem! [ha : Inhabited α] : mkList xs.length (xs[·]!) = xs := by
+  simp [mkList]
+
+-- #check 0 #exit
+
+end List
+
+namespace Std.ExtDHashMap
+
+open Std
+
+variable {α : Type*} {β : α → Type*} {γ : α → Type*}
+variable [hh₁ : DecidableEq α] [hh₂ : Hashable α]
+variable {mp mp₁ mp₂ m m₁ m₂ m₃ : ExtDHashMap α β}
+variable [ha : LinearOrder α]
+omit ha
+
+attribute [simp] keys_empty
+
+include ha in
+theorem toList_insert_of_not_mem {i x} (h : i ∉ m) : (m.insert i x).toList =
+(⟨i, x⟩ :: m.toList).mergeSort (·.1 ≤ ·.1) := by
+  rw [List.eq_iff_of_nodup_and_pairwise (r := (·.1 ≤ ·.1))]
+  rotate_left
+  · simp
+  · simp [get?_eq_none_of_not_mem h]
+  · rintro ⟨j, y⟩ ⟨k, z⟩
+    simp; grind
+  · simp
+  · have h₁ := @List.pairwise_mergeSort
+    specialize @h₁ ((i : α) × β i) (le := (·.1 ≤ ·.1))
+      (by simp) (by simp) (⟨i, x⟩ :: m.toList)
+    grind
+  rintro ⟨j, y⟩; simp
+  by_cases h₁ : j = i
+  · subst h₁; simp [eq_comm, get?_eq_none_of_not_mem h]
+  simp [h₁, get?_insert, ne_symm' h₁]
+
+include ha in
+theorem keys_insert_of_not_mem {i x} (h : i ∉ m) :
+(m.insert i x).keys = (i :: m.keys).mergeSort := by
+  simp [keys_eq_map_fst_toList, toList_insert_of_not_mem h]
+  apply List.eq_of_sortedLE_and_perm
+  · rw [List.map_mergeSort (s := (· ≤ ·)) (by simp)]
+    apply List.sortedLE_mergeSort
+  · apply List.sortedLE_mergeSort
+  simp
+  rw [List.perm_iff_mem_iff_of_nodup]; simp
+  on_goal 2 => simpa [←keys_eq_map_fst_toList]
+  rw [List.nodup_map_iff_inj_on]
+  rotate_left
+  · simp [get?_eq_none_of_not_mem h]
+  simp
+  split_ands
+  · rintro ⟨j, y⟩ h₁ rfl
+    simp [get?_eq_none_of_not_mem h] at h₁
+  rintro ⟨j, y⟩ h₁
+  dsimp at h₁ ⊢
+  split_ands
+  · rintro rfl; simp [get?_eq_none_of_not_mem h] at h₁
+  · grind
+
+@[simp]
+theorem get?_out_inner {i} : m.inner.out.get? i = m.get? i := by
+  rcases m with ⟨m⟩
+  induction m using Quotient.inductionOn
+  simp [get?, lift]
+
+@[simp]
+theorem get?_mk {m i} : ({inner := m} : ExtDHashMap α β).get? i = m.out.get? i := by
+  simp [get?, lift, Quotient.lift_eq]
+
+@[simp]
+theorem insert_mk {m i x} :
+({inner := m} : ExtDHashMap α β).insert i x = {inner := ⟦m.out.insert i x⟧} := by
+  simp [insert, lift, Quotient.lift_eq]
+
+@[simp]
+theorem erase_mk {m i} :
+({inner := m} : ExtDHashMap α β).erase i = {inner := ⟦m.out.erase i⟧} := by
+  simp [erase, lift, Quotient.lift_eq]
+
+@[simp]
+theorem insert_erase_eq_self_iff {i x} :
+(m.erase i).insert i x = m ↔ m.get? i = some x := by
+  constructor <;> intro h
+  · rw [←h]; simp
+  rw [ext_iff']
+  have h₁ := @DHashMap.insert_erase_equiv
+  specialize @h₁ α β _ _ m.inner.out i x _
+  · simpa
+  symm; apply h₁.symm.trans; symm; clear h₁
+  change (_ : DHashMap α β) ≈ _
+  rw [←Quotient.eq_mk_iff_out]
+  rcases m with ⟨m⟩
+  simp at h ⊢
+  apply DHashMap.equiv_iff_get?.mpr
+  intro j
+  ext y
+  simp [DHashMap.get?_insert]
+
+include ha in @[simp]
+theorem keys_eq_keys_iff {m₁ : ExtDHashMap α β} {m₂ : ExtDHashMap α γ} :
+m₁.keys = m₂.keys ↔ ∀ i, i ∈ m₁ ↔ i ∈ m₂ := by
+  induction m₂ using ind generalizing m₁
+  · simp [eq_empty_iff]
+  nm m₂ i x h₁ ih
+  simp
+  rw [keys_insert_of_not_mem h₁]
+  constructor
+  · intro h₂ j
+    replace h₂ := congrArg (j ∈ ·) h₂
+    simp at h₂
+    tauto
+  intro h₂
+  have h₃ : i ∈ m₁; grind
+  clear x
+  obtain ⟨x, h₄⟩ := get?_eq_some_of_mem h₃
+  have h₅ : m₁ = (m₁.erase i).insert i x
+  · symm; simpa
+  rw [h₅]
+  rw [keys_insert_of_not_mem (by simp)]
+  rw [List.mergeSort_eq_mergeSort_iff (by simp) (by simp) (by simp)]
+  simp; rw [List.perm_iff_mem_iff_of_nodup (by simp) (by simp)]; grind
+
+-- #check 0 #exit
+
+end Std.ExtDHashMap
+
+namespace Map
+
+open Std
+
+universe u v w
+variable {α : Type u} {β : Type v} {γ : Type w}
+variable [hh₁ : DecidableEq α] [hh₂ : Hashable α]
+variable {mp m m₁ m₂ m₃ : Map α β}
+variable [ha : LinearOrder α]
+omit ha
+
+theorem get!_insert [hb : Inhabited β] {i x j} :
+(mp.insert i x).get! j = if j = i then x else mp.get! j := by
+  simp [get!_eq_get!_get?, get?_insert]; grind
+
+theorem get?_ofList_eq_some_iff {xs : List (α × β)} {i x}
+(h : (xs.map (·.1)).Nodup) : (ofList xs).get? i = some x ↔ ⟨i, x⟩ ∈ xs := by
+  simp [ofList]; rw [ExtDHashMap.get?_ofList_eq_some_iff (by simpa)]; simp
+
+theorem get?_ofList_of_nodup {xs : List (α × β)} {i} (h : (xs.map (·.1)).Nodup) :
+(ofList xs).get? i = (xs.find? (·.fst = i)).map (·.2) := by
+  unfold Option.map; split
+  · nm a x h₁; clear a
+    rename' i => j
+    rcases x with ⟨i, x⟩
+    rw [get?_ofList_eq_some_iff h]
+    grind
+  nm a h₁; clear a
+  simp at h₁ ⊢
+  grind
+
+theorem get!_ofList_of_nodup [hb : Inhabited β] {xs : List (α × β)} {i}
+(h : (xs.map (·.1)).Nodup) : (ofList xs).get! i =
+((xs.find? (·.fst = i)).map (·.2)).get! := by
+  rw [get!_eq_get!_get?, get?_ofList_of_nodup h]
+
+@[simp]
+theorem mem_union {i} : i ∈ m₁ ∪ m₂ ↔ i ∈ m₁ ∨ i ∈ m₂ := by
+  simp [mem_iff_get?_eq_some, get?_union]; grind
+
+include ha in @[simp]
+theorem keys_mk {mp} : (⟨mp⟩ : Map α β).keys = mp.keys := rfl
+
+@[simp]
+theorem insert_mk {m i x} : (⟨m⟩ : Map α β).insert i x = ⟨m.insert i x⟩ := rfl
+
+@[simp]
+theorem erase_mk {m i} : (⟨m⟩ : Map α β).erase i = ⟨m.erase i⟩ := rfl
+
+include ha in
+theorem toList_insert_of_not_mem {i x} (h : i ∉ m) : (m.insert i x).toList =
+(⟨i, x⟩ :: m.toList).mergeSort (·.1 ≤ ·.1) := by
+  rcases m with ⟨m⟩; simp at h ⊢
+  rw [ExtDHashMap.toList_insert_of_not_mem h]
+  rw [List.map_mergeSort (s := (·.1 ≤ ·.1)) (by simp)]
+  simp
+
+include ha in
+theorem keys_insert_of_not_mem {i x} (h : i ∉ m) :
+(m.insert i x).keys = (i :: m.keys).mergeSort := by
+  rcases m with ⟨m⟩; simp at h ⊢
+  rw [ExtDHashMap.keys_insert_of_not_mem h]
+
+@[simp]
+theorem insert_erase_eq_self_iff {i x} :
+(m.erase i).insert i x = m ↔ m.get? i = some x := by
+  rcases m with ⟨m⟩; simp
+
+include ha in @[simp]
+theorem keys_eq_keys_iff {m₁ : Map α β} {m₂ : Map α γ} :
+m₁.keys = m₂.keys ↔ ∀ i, i ∈ m₁ ↔ i ∈ m₂ := by
+  rcases m₁, m₂ with ⟨⟨m₁⟩, ⟨m₂⟩⟩; simp
+
+theorem union_assoc : (m₁ ∪ m₂) ∪ m₃ = m₁ ∪ (m₂ ∪ m₃) := by
+  simp [ext_iff, get?_union]; grind
+
+@[simp]
+theorem union_self : m ∪ m = m := by
+  simp [ext_iff, get?_union]
+
+@[simp]
+theorem union_union_self : m₁ ∪ (m₁ ∪ m₂) = m₁ ∪ m₂ := by
+  simp [←union_assoc]
+
+def diff (m₁ m₂ : Map α β) : Map α β :=
+  ⟨m₁.1 \ m₂.1⟩
+
+instance : SDiff (Map α β) := ⟨diff⟩
+theorem diff_def : m₁ \ m₂ = m₁.diff m₂ := rfl
+
+@[simp]
+theorem mk_diff_mk {m₁ m₂} : (⟨m₁⟩ : Map α β) \ ⟨m₂⟩ = ⟨m₁ \ m₂⟩ := rfl
+
+theorem get?_diff {i} : (m₁ \ m₂).get? i = if i ∈ m₂ then none else m₁.get? i := by
+  rcases m₁, m₂ with ⟨⟨m₁⟩, ⟨m₂⟩⟩; simp [ExtDHashMap.get?_diff]
+
+@[simp]
+theorem union_diff_self : m₁ ∪ (m₂ \ m₁) = m₂ ∪ m₁ := by
+  simp [ext_iff, get?_union, get?_diff]
+  intro i
+  rw! (castMode := .all) [mem_iff_get?_eq_some]
+  split_ifs with h; grind
+  simp at h
+  rw [←Option.eq_none_iff_forall_ne_some] at h
+  grind
+
+theorem union_eq_self_left_iff : m₁ ∪ m₂ = m₁ ↔
+∀ i x, m₂.get? i = some x → m₁.get? i = some x := by
+  simp [ext_iff, get?_union, Option.or]; grind
+
+@[simp]
+theorem union_insert_empty {i x} : m₁ ∪ (∅ : Map α β).insert i x = m₁.insert i x := by
+  simp [ext_iff, get?_union, get?_insert]; grind
+
+-- #check 0 #exit
+
+end Map
+
 namespace Esolangs.Cornucopia
+
+structure CompatibleDefs (defs : Map String Def) (fs : Map String (List ℕ → ℕ)) : Prop where
+  keys_fs : fs.keys = defs.keys
+  eval_of_ne_arity ⦃name d⦄ : defs.get? name = some d → ∀ ⦃xs : List ℕ⦄,
+    xs.length ≠ d.arity → fs.get! name xs = 0
+  eval_eq ⦃name d⦄ : defs.get? name = some d → ∀ ⦃xs : List ℕ⦄,
+    xs.length = d.arity → fs.get! name xs = d.expr.eval
+    ⟨builtinDefs ∪ .ofList defs.toList⟩ (builtinFs ∪ fs) xs
+
+structure WFDefs (defs : List (String × Def)) : Prop where
+  nodup_names : defs.map (·.1) |>.Nodup
+  not_isBuiltin_of_mem ⦃name d⦄ : (name, d) ∈ defs → ¬IsBuiltin name
+  wf_main : ∃ d, (mainName, d) ∈ defs ∧ d.arity = 1
+  wf_def ⦃name d⦄ : (name, d) ∈ defs → d.WF (Prog.ofDefs defs)
+  exiu_compatible : ∃! fs, CompatibleDefs (.ofList defs) fs
+
+-- #check 0 #exit
 
 def exprId : Expr :=
   .arg 0
 
-def progId : Prog where
-  defs := [⟨1, exprId⟩]
+def exprLoop (name : String) : Expr :=
+  .call name [.arg 0]
 
-def exprLoop (i : ℕ) : Expr :=
-  .call (.custom i) [.arg 0]
+def progId : Prog :=
+  .ofDefs [(mainName, ⟨1, exprId⟩)]
 
-def progLoop : Prog where
-  defs := [⟨1, exprLoop 0⟩]
+def progLoop : Prog :=
+  .ofDefs [(mainName, ⟨1, exprLoop mainName⟩)]
 
 -- #check 0 #exit
 
 -----
 
-@[simp] theorem defs_progId : progId.defs = [⟨1, exprId⟩] := rfl
-@[simp] theorem main_progId : progId.main = ⟨1, exprId⟩ := rfl
+@[simp]
+theorem mem_builtins {b} : b ∈ builtins := by
+  cases b <;> decide
+
+instance {name} : Decidable (IsBuiltin name) :=
+  decidable_of_bool (name ∈ builtinDefs) # by simp [IsBuiltin, builtinDefs]
+
+@[simp] theorem def_mk {defs name} : (Prog.mk defs).def name = defs.get! name := rfl
+@[simp] theorem def?_mk {defs name} : (Prog.mk defs).def? name = defs.get? name := rfl
+@[simp] theorem main_mk {defs} : (Prog.mk defs).main = defs.get! mainName := rfl
+@[simp] theorem Prog.defs_mk {ds} : defs ⟨ds⟩ = ds := rfl
+@[simp] theorem Builtin.arity_succ : Builtin.succ.arity = 1 := rfl
+@[simp] theorem Builtin.arity_sub : Builtin.sub.arity = 2 := rfl
+@[simp] theorem Prog.arity_mk {defs name} : arity ⟨defs⟩ name = (defs.get! name).arity := rfl
+@[simp] theorem Prog.expr_mk {defs name} : expr ⟨defs⟩ name = (defs.get! name).expr := rfl
+
+@[simp]
+theorem mem_builtinDefs {name} : name ∈ builtinDefs ↔ IsBuiltin name := by
+  simp [builtinDefs, IsBuiltin]
+
+@[simp]
+theorem not_isBuiltin_mainName : ¬IsBuiltin mainName := by
+  simp [IsBuiltin]; decide
+
+theorem Prog.def_ofDefs {xs name} (h : ¬IsBuiltin name) :
+(Prog.ofDefs xs).def name = (Map.ofList xs).get! name := by
+  simp [ofDefs]; rw [Map.get!_union_right]; simpa
+
+theorem arity_ofDefs {defs name} (h : ¬IsBuiltin name) :
+(Prog.ofDefs defs).arity name = ((Map.ofList defs).get! name).arity := by
+  simp [Prog.arity, Prog.def_ofDefs h]
+
+@[simp]
+theorem Prog.main_ofDefs {xs} : (Prog.ofDefs xs).main = (Map.ofList xs).get! mainName := by
+  simp [ofDefs]; rw [Map.get!_union_right]; simp
+
+@[simp]
+theorem main_progId : progId.main = ⟨1, exprId⟩ := by
+  simp [progId, Map.get!_insert]
+
+@[simp]
+theorem main_progLoop : progLoop.main = ⟨1, exprLoop mainName⟩ := by
+  simp [progLoop, Map.get!_insert]
+
 @[simp] theorem wf_exprId {prog} : exprId.WF prog 1 := by simp [Expr.WF, exprId]
 @[simp] theorem wf_defId : (Def.mk 1 (.arg 0)).WF progId := wf_exprId
-@[simp] theorem arity_zero_progId : progId.arity 0 = 1 := rfl
-@[simp] theorem expr_zero_progId : progId.expr 0 = exprId := rfl
 
 @[simp]
 theorem Expr.run_arg {i prog f args} : (arg i).eval prog f args = args[i]! := by
   simp [eval]
 
-@[simp] theorem Prog.defs_mk {ds} : defs ⟨ds⟩ = ds := rfl
-@[simp] theorem Builtin.arity_succ : Builtin.succ.arity = 1 := rfl
-@[simp] theorem Builtin.arity_sub : Builtin.sub.arity = 2 := rfl
-@[simp] theorem Prog.arity_mk {defs i} : arity ⟨defs⟩ i = defs[i]!.arity := rfl
-@[simp] theorem Prog.expr_mk {defs i} : expr ⟨defs⟩ i = defs[i]!.expr := rfl
-@[simp] theorem Target.f_custom {fs i} : (custom i).f fs = fs[i]! := rfl
-@[simp] theorem Target.arity_custom {prog i} : (custom i).arity prog = prog.arity i := rfl
-@[simp] theorem Prog.main_mk {defs} : main ⟨defs⟩ = defs[0]! := rfl
-
 @[simp]
 theorem Expr.wf_arg {prog n i} : (arg i).WF prog n ↔ i < n := by
   simp [WF]
 
+@[simp]
+theorem Builtin.isBuiltin {b : Builtin} : IsBuiltin b.name := by
+  simp [IsBuiltin]
+
+@[simp]
+theorem nodup_builtins : builtins.Nodup := by
+  decide
+
+@[simp]
+theorem nodup_map_name_builtins : (builtins.map Builtin.name).Nodup := by
+  decide
+
+@[simp]
+theorem Builtin.get?_builtinDefs {b : Builtin} : builtinDefs.get? b.name = some b.def := by
+  simp [builtinDefs, Map.get?_ofList_eq_some_iff]; use b
+
+@[simp]
+theorem Builtin.get!_builtinDefs {b : Builtin} : builtinDefs.get! b.name = b.def := by
+  simp [Map.get!_eq_get!_get?]
+
+theorem def?_ofDefs_builtin_eq_of {defs} {b : Builtin}
+(h : ∀ d ∈ defs, ¬IsBuiltin d.1) : (Prog.ofDefs defs).def? b.name = some b.def := by
+  simp [Prog.ofDefs]; rw [Map.get?_union_left]; simp
+  simp; intro d h₁; specialize h _ h₁; simp at h
+
+@[simp]
+theorem Prog.defs_ofDefs {defs} : (Prog.ofDefs defs).defs = builtinDefs ∪ .ofList defs := rfl
+
+@[simp]
+theorem Prog.hasDef_ofDefs {defs name} :
+(Prog.ofDefs defs).HasDef name ↔ IsBuiltin name ∨ name ∈ Map.ofList defs := by
+  simp [HasDef]
+
+@[simp]
+theorem Builtin.ext_name {b₁ b₂ : Builtin} : b₁.name = b₂.name ↔ b₁ = b₂ := by
+  rcases b₁, b₂ with ⟨⟨⟩, ⟨⟩⟩ <;> decide
+
+@[simp] theorem Builtin.arity_def {b : Builtin} : b.def.arity = b.arity := rfl
+@[simp] theorem Builtin.expr_def {b : Builtin} : b.def.expr = b.expr := rfl
+
+@[simp]
+theorem Builtin.ext_def {b₁ b₂ : Builtin} : b₁.def = b₂.def ↔ b₁ = b₂ := by
+  rcases b₁, b₂ with ⟨⟨⟩, ⟨⟩⟩ <;> simp [Def.ext_iff]
+
+@[simp]
+theorem get?_builtinDefs_eq_some {name d} :
+builtinDefs.get? name = some d ↔ ∃ (b : Builtin), b.name = name ∧ b.def = d := by
+  simp [builtinDefs, Map.get?_ofList_of_nodup]
+  apply exists_congr; intro b; simp; rintro rfl
+  rw [List.find?_eq_some_iff_of_at_most_one]; simp
+  simp; rintro b₁ b₂ rfl; simp [eq_comm]
+
+@[simp]
+theorem Builtin.wf_expr {prog} {b : Builtin} :
+b.expr.WF prog b.arity ↔ ∃ d, prog.def? b.name = some d ∧ d.arity = b.arity := by
+  simp [expr, Expr.WF, Prog.HasDef, Map.mem_iff_get?_eq_some,
+    Prog.arity, Prog.def, Map.get!_eq_get!_get?, Prog.def?]
+  grind
+
+theorem WFDefs.not_mem_of_isBuiltin {defs name d} (H : WFDefs defs)
+(h : IsBuiltin name) : (name, d) ∉ defs := by
+  grind [H.not_isBuiltin_of_mem]
+
+theorem WFDefs.not_mem_builtin {defs} {b : Builtin} {d}
+(H : WFDefs defs) : (b.name, d) ∉ defs := by
+  apply H.not_mem_of_isBuiltin; simp
+
+theorem WFDefs.get?_ofList_defs {defs name d} (H : WFDefs defs) :
+(Map.ofList defs).get? name = some d ↔ (name, d) ∈ defs :=
+  Map.get?_ofList_eq_some_iff H.nodup_names
+
+@[simp]
+theorem Builtin.get?_namesMap {b : Builtin} : namesMap.get? b.name = some b := by
+  simp [namesMap]; rw [Map.get?_ofList_of_nodup (by simp)]; simp
+  rw [List.find?_eq_some_iff_of_at_most_one] <;> simp
+
+@[simp]
+theorem Builtin.get!_namesMap {b : Builtin} : namesMap.get! b.name = b := by
+  simp [Map.get!_eq_get!_get?]
+
+theorem Builtin.name_get!_namesMap_of_isBuiltin {name} (h : IsBuiltin name) :
+(namesMap.get! name).name = name := by
+  obtain ⟨b, rfl⟩ := h; simp
+
+theorem WFDefs.isBuiltin_or {defs name d} (H : WFDefs defs)
+(h : (builtinDefs ∪ .ofList defs).get? name = some d) :
+IsBuiltin name ∨ (name, d) ∈ defs := by
+  rw [or_iff_not_imp_left]
+  intro h₂
+  rw [Map.get?_union_right (by simpa)] at h
+  rw [H.get?_ofList_defs] at h
+  exact h
+
+theorem WFDefs.hasDef {defs name d} (H : WFDefs defs)
+(h : (builtinDefs ∪ .ofList defs).get? name = some d) :
+(Prog.ofDefs defs).HasDef name := by
+  have := H.isBuiltin_or h; simp; tauto
+
+theorem Prog.def_eq_get!_def? {prog : Prog} {name} :
+prog.def name = (prog.def? name).get! := by
+  simp [Prog.def, Prog.def?, Map.get!_eq_get!_get?]
+
+theorem Prog.def?_of_get? {defs name d}
+(h : (builtinDefs ∪ .ofList defs).get? name = some d) :
+(Prog.ofDefs defs).def? name = some d := by
+  simpa [Prog.ofDefs]
+
+theorem Prog.def_of_get? {defs name d}
+(h : (builtinDefs ∪ .ofList defs).get? name = some d) :
+(Prog.ofDefs defs).def name = d := by
+  simp [Prog.def_eq_get!_def?, def?_of_get? h]
+
+theorem Prog.arity_of_get? {defs name d}
+(h : (builtinDefs ∪ .ofList defs).get? name = some d) :
+(Prog.ofDefs defs).arity name = d.arity := by
+  simp [arity, def_of_get? h]
+
+theorem Prog.expr_of_get? {defs name d}
+(h : (builtinDefs ∪ .ofList defs).get? name = some d) :
+(Prog.ofDefs defs).expr name = d.expr := by
+  simp [expr, def_of_get? h]
+
+theorem WFDefs.get?_builtin {defs} {b : Builtin} (H : WFDefs defs) :
+(builtinDefs ∪ .ofList defs).get? b.name = some b.def := by
+  rw [Map.get?_union_left # by simp [H.not_mem_builtin]]; simp
+
+theorem WFDefs.get?_of_mem_defs {defs} (H : WFDefs defs) {name d}
+(h : (name, d) ∈ defs) : (builtinDefs ∪ .ofList defs).get? name = some d := by
+  rw [Map.get?_union_right # by simp [H.not_isBuiltin_of_mem h]]
+  rw [Map.get?_ofList_of_nodup H.nodup_names]
+  simp; use name
+  rw [List.find?_eq_some_iff_of_at_most_one]; grind
+  rintro ⟨name₁, d₁⟩ ⟨name₂, d₂⟩ h₁ h₂
+  simp
+  rintro rfl rfl
+  simp
+  have h₃ := H.nodup_names
+  rw [List.nodup_map_iff_inj_on # List.Nodup.of_map _ h₃] at h₃
+  grind
+
+theorem WFDefs.def?_builtin {defs} {b : Builtin} (H : WFDefs defs) :
+(Prog.ofDefs defs).def? b.name = some b.def := by
+  simp [Prog.ofDefs, H.get?_builtin]
+
+theorem WFDefs.def_builtin {defs} {b : Builtin} (H : WFDefs defs) :
+(Prog.ofDefs defs).def b.name = b.def := by
+  simp [Prog.def_eq_get!_def?, H.def?_builtin]
+
+theorem WFDefs.arity_builtin {defs} {b : Builtin} (H : WFDefs defs) :
+(Prog.ofDefs defs).arity b.name = b.arity := by
+  simp [Prog.arity, H.def_builtin]
+
+theorem WFDefs.expr_builtin {defs} {b : Builtin} (H : WFDefs defs) :
+(Prog.ofDefs defs).expr b.name = b.expr := by
+  simp [Prog.expr, H.def_builtin]
+
+theorem WFDefs.def?_of_mem_defs {defs name d} (H : WFDefs defs)
+(h : (name, d) ∈ defs) : (Prog.ofDefs defs).def? name = some d :=
+  H.get?_of_mem_defs h
+
+theorem WFDefs.def_of_mem_defs {defs name d} (H : WFDefs defs)
+(h : (name, d) ∈ defs) : (Prog.ofDefs defs).def name = d := by
+  simp [Prog.def_eq_get!_def?, H.def?_of_mem_defs h]
+
+theorem WFDefs.arity_of_mem_defs {defs name d} (H : WFDefs defs)
+(h : (name, d) ∈ defs) : (Prog.ofDefs defs).arity name = d.arity := by
+  simp [Prog.arity, H.def_of_mem_defs h]
+
+theorem WFDefs.expr_of_mem_defs {defs name d} (H : WFDefs defs)
+(h : (name, d) ∈ defs) : (Prog.ofDefs defs).expr name = d.expr := by
+  simp [Prog.expr, H.def_of_mem_defs h]
+
+@[simp]
+theorem mem_builtinFS {name} : name ∈ builtinFs ↔ IsBuiltin name := by
+  simp [builtinFs, IsBuiltin]
+
+theorem WFDefs.builtin_not_mem_defs {defs} {b : Builtin} {d}
+(H : WFDefs defs) : (b.name, d) ∉ defs := by
+  intro h; replace h := H.not_isBuiltin_of_mem h; simp at h
+
+@[simp]
+theorem Builtin.get?_builtinFs {b : Builtin} : builtinFs.get? b.name = some b.eval := by
+  simp [builtinFs]; rw [Map.get?_ofList_eq_some_iff] <;> simp
+
+@[simp]
+theorem Builtin.get!_builtinFs {b : Builtin} : builtinFs.get! b.name = b.eval := by
+  simp [Map.get!_eq_get!_get?]
+
+theorem Builtin.eval_of_ne_arity {b : Builtin} {xs}
+(h : xs.length ≠ b.arity) : b.eval xs = 0 := by
+  simp at h ⊢; simp [Builtin.eval, fn, h]
+
+theorem CompatibleDefs.get?_builtin {defs fs} {b : Builtin} (H : WFDefs defs)
+(H₁ : CompatibleDefs (.ofList defs) fs) : (builtinFs ∪ fs).get? b.name = some b.eval := by
+  have h₃ := H₁.keys_fs; simp at h₃
+  rw [Map.get?_union_left]; simp
+  simp [h₃]; intro d; apply H.builtin_not_mem_defs
+
+theorem CompatibleDefs.get!_builtin {defs fs} {b : Builtin} (H : WFDefs defs)
+(H₁ : CompatibleDefs (.ofList defs) fs) : (builtinFs ∪ fs).get! b.name = b.eval := by
+  simp [Map.get!_eq_get!_get?, H₁.get?_builtin H]
+
+@[simp]
+theorem Builtin.eval_mkList {b : Builtin} {xs} :
+b.eval (mkList b.arity (xs[·]!)) = b.info.eval xs := by
+  simp [eval, fn]; cases b <;> simp [Builtin.info]
+
+@[simp]
+theorem get?_builtinFs_eq_some {name f} : builtinFs.get? name = some f ↔
+∃ (b : Builtin), b.name = name ∧ b.eval = f := by
+  simp [builtinFs, Map.get?_ofList_eq_some_iff]
+
+theorem Prog.WF.def_builtin  {prog : Prog} {b : Builtin} [H : prog.WF] :
+prog.def b.name = b.def := by
+  simp [def_eq_get!_def?, H.def?_builtin]
+
+@[simp]
+theorem Builtin.name_ne_mainName {b : Builtin} : b.name ≠ mainName := by
+  cases b <;> decide
+
+@[simp]
+theorem Builtin.mainName_ne_name {b : Builtin} : mainName ≠ b.name :=
+  ne_symm' b.name_ne_mainName
+
+-- #check 0 #exit
+
+-- theorem Prog.Compatible.get?_builtin_ofDefs {defs} {b : Builtin} {fs}
+-- (H₁ : (Prog.ofDefs defs).Compatible fs) : fs.get? b.name = some b.eval := by
+--   have h₁ := @H₁.eval_eq b.name
+--   specialize @h₁ (by simp) (mkList b.arity id) _
+--   ·
+--     clear h₁
+--     cases H
+--     simp [arity, H.def_builtin]
+
+-- #check 0 #exit
+
+-- theorem Prog.Compatible.builtinFs_union {defs fs} (H : (Prog.ofDefs defs).WF)
+-- (H₁ : (Prog.ofDefs defs).Compatible fs) : fs ∪ builtinFs = fs := by
+--   rw [Map.union_eq_self_left_iff]
+--   intro name f h
+--   simp at h
+--   obtain ⟨b, rfl, rfl⟩ := h
+--   exact H₁.get?_builtin H
+
+example : ¬∀ {defs} (H : WFDefs defs),
+∃! fs, (Prog.ofDefs defs).Compatible fs := by
+  simp [not_exiu_iff]
+  use [(mainName, ⟨1, exprId⟩)]
+  split_ands
+  ·
+    constructor <;> simp
+    use .ofList [(mainName, fn 1 (·[0]!))]
+    simp
+    split_ands
+    ·
+      constructor <;> simp [Map.get?_insert, Map.get!_eq_get!_get?, fn, exprId]
+    ·
+      intro fs
+      rintro ⟨h₁, h₂, h₃⟩
+      simp [Map.get?_insert, Map.get!_eq_get!_get?, exprId] at h₁ h₂ h₃
+      simp [Map.ext_iff, Map.get?_insert]
+      intro name
+      rw! (castMode := .all) [eq_comm (a := mainName)]
+      split_ifs with h₄
+      rotate_left
+      ·
+        simp [←h₁] at h₄
+        simpa
+      subst h₄
+      specialize h₁ mainName
+      simp at h₁
+      rw [Map.mem_iff_get?_eq_some] at h₁
+      choose f h₁ using h₁
+      ext xs
+      simp [h₁]
+      unfold fn
+      simp
+      revert xs
+      simp
+      ext xs
+      split_ifs with h₄
+      ·
+        specialize h₃ h₄
+        simp [h₁] at h₃
+        rw [h₃]
+      ·
+        specialize h₂ h₄
+        simp [h₁] at h₂
+        rw [h₂]
+  
+  intro fs h
+  use fs.insert Builtin.succ.name # fn 1 # λ xs =>
+    fs.get! Builtin.succ.name xs + 1
+  split_ands
+  ·
+    obtain ⟨h₂, h₃, h₄⟩ := h
+    simp at h₂ h₃ h₄
+    constructor <;> simp
+    ·
+      intro name
+      simp [h₂]
+      rintro rfl
+      simp
+    ·
+      rintro name (⟨b, rfl⟩ | rfl) xs h
+      ·
+        specialize @h₃ b.name (by simp) xs h
+        simp [Prog.arity, Prog.ofDefs, Map.get!_insert] at h
+        simp [Map.get!_insert]
+        split_ifs with h₅
+        · subst h₅
+          simp at h
+          simp [fn, h]
+        · exact h₃
+      ·
+        simp [Map.get!_insert]
+        exact h₃ (by simp) h
+    ·
+      rintro name (⟨b, rfl⟩ | rfl) xs h
+      ·
+        simp [Map.get!_insert, Prog.expr, Prog.ofDefs] at h ⊢
+        split_ifs with h₅
+        ·
+          subst h₅
+          simp at h
+          simp [fn, h, Builtin.expr, Expr.eval, Map.get!_insert]
+          rw [←h]; simp
+        ·
+          simp [Builtin.expr, Expr.eval, Map.get!_insert, h₅, ←h]
+      ·
+        specialize @h₄ mainName (by simp) xs h
+        simp [Map.get!_insert, Prog.expr, Prog.ofDefs] at h ⊢
+        simp [exprId]
+        rw [h₄]
+        simp [Prog.ofDefs, Map.get!_insert, exprId]
+  
+  ·
+    apply ne_of_congr (·.get! Builtin.succ.name)
+    simp [Map.get!_insert, funext_iff]
+    use [0]
+    simp [fn]
+
+#check 0 #exit
+
+theorem WFDefs.compatible_fs {defs} (H : WFDefs defs) :
+∃! fs, (Prog.ofDefs defs).Compatible fs := by
+  obtain ⟨fs, H₁, H₂⟩ := H.exiu_compatible
+  dsimp at H₂
+  use builtinFs ∪ fs
+  dsimp; split_ands
+  · constructor
+    ·
+      simp
+      intro name h₁
+      have h₂ := H₁.keys_fs
+      simp at h₂
+      apply h₂
+    · intro name h₁ xs h₂
+      simp at h₁
+      have h₃ := H₁.keys_fs
+      simp at h₃
+      specialize h₃ name
+      rw [←h₃] at h₁
+      rcases h₁ with ⟨b, rfl⟩ | h₁
+      · rw [H₁.get!_builtin H]
+        rw [H.arity_builtin] at h₂
+        exact b.eval_of_ne_arity h₂
+      rw [h₃] at h₁
+      choose d h₁ using h₁
+      rw [H.arity_of_mem_defs h₁] at h₂
+      have h₄ := @H₁.eval_of_ne_arity name
+      specialize @h₄ d _ xs h₂
+      · rwa [Map.get?_ofList_eq_some_iff H.nodup_names]
+      rwa [Map.get!_union_right]
+      simp [H.not_isBuiltin_of_mem h₁]
+    ·
+      intro name h₁ xs h₂
+      simp at h₁
+      have h₃ := H₁.keys_fs
+      simp at h₃
+      rcases h₁ with ⟨b, rfl⟩ | ⟨d, h₁⟩
+      ·
+        rw [H₁.get!_builtin H]
+        simp [H.arity_builtin] at h₂
+        simp [H.expr_builtin, Builtin.eval, fn, h₂, Builtin.expr, Expr.eval]
+        simp [H₁.get!_builtin H]
+      rw [Map.get!_union_right # by simp [H.not_isBuiltin_of_mem h₁]]
+      rw [H.expr_of_mem_defs h₁]
+      rw [H.arity_of_mem_defs h₁] at h₂
+      have h₄ := @H₁.eval_eq
+      specialize @h₄ name d _ xs h₂
+      · rwa [Map.get?_ofList_eq_some_iff H.nodup_names]
+      convert h₄
+      simp [Prog.ext_iff]
+  ·
+    intro fs' h₁
+    specialize H₂ (fs' \ builtinFs) _
+    ·
+      sorry
+    subst H₂
+    symm; simp [Map.union_eq_self_left_iff]
+    rintro name b rfl
+    have h₂ := @h₁.eval_eq
+    specialize @h₂ b.name (by simp) (mkList b.arity id) _
+    ·
+      clear h₂
+      simp
+
+#check 0 #exit
+
+    -- constructor
+    -- · simp [H₁.keys_fs]
+    -- · intro name h₁ xs h₂
+    --   simp at h₁; rcases h₁ with ⟨b, rfl⟩ | ⟨d, h₁⟩
+    --   · apply H₁.eval_of_ne_arity (d := b.def) H.get?_builtin
+    --     contrapose! h₂
+    --     rw [h₂, Prog.arity_of_get? H.get?_builtin]
+    --   have h₃ := H.get?_of_mem_defs h₁
+    --   apply H₁.eval_of_ne_arity h₃
+    --   contrapose! h₂
+    --   rw [h₂, Prog.arity_of_get? h₃]
+    -- · intro name h₁ xs h₂
+    --   simp at h₁; rcases h₁ with ⟨b, rfl⟩ | ⟨d, h₁⟩
+    --   · have h₃ := @H₁.eval_eq b.name b.def H.get?_builtin xs
+    --     simp [Prog.arity_of_get? H.get?_builtin] at h₂
+    --     simp [h₂] at h₃
+    --     simp [H.expr_builtin]
+    --     convert h₃
+    --     simp [Prog.ext_iff]
+    --   simp [H.expr_of_mem_defs h₁]
+    --   simp [H.arity_of_mem_defs h₁] at h₂
+    --   convert @H₁.eval_eq name d (H.get?_of_mem_defs h₁) xs h₂
+    --   simp [Prog.ext_iff]
+
+#check 0 #exit
+
+theorem WFDefs.wf {defs} (H : WFDefs defs) : (Prog.ofDefs defs).WF := by
+  constructor
+  · intro b
+    simp [Prog.ofDefs]
+    rw [Map.get?_union_left]; simp
+    simp [H.not_mem_of_isBuiltin]
+  · simp; grind [H.wf_main]
+  · obtain ⟨d, h₁, h₂⟩ := H.wf_main
+    have h₃ := H.nodup_names
+    simp [Map.get!_ofList_of_nodup h₃]
+    unfold Option.map
+    split
+    · nm a x h; clear a
+      rw [List.nodup_map_iff_inj_on # List.Nodup.of_map _ h₃] at h₃
+      rw [List.find?_eq_some_iff_of_at_most_one] at h
+      rotate_left
+      · rintro ⟨name₁, d₁⟩ ⟨name₂, d₂⟩ h₄ h₅
+        simp
+        rintro rfl rfl
+        simp
+        grind
+      simp at h ⊢
+      obtain ⟨d₁, h₄⟩ := H.wf_main
+      rcases x with ⟨name, x⟩
+      dsimp at *
+      rcases h with ⟨h, rfl⟩
+      grind
+    · grind
+  · intro name d h₁
+    have h := @H.wf_def name d
+    simp [Prog.ofDefs] at h₁
+    by_cases h₂ : IsBuiltin name
+    · clear h
+      have h₀ := λ d => H.not_mem_of_isBuiltin h₂ (d := d)
+      rw [Map.get?_union_left # by simp [h₀]] at h₁
+      simp at h₁
+      obtain ⟨b, rfl, rfl⟩ := h₁
+      simp [Def.WF]
+      use b.def
+      simp [Prog.ofDefs]
+      rw [Map.get?_union_left # by simp [h₀]]
+      simp
+    rw [Map.get?_union_right (by simpa)] at h₁
+    rw [Map.get?_ofList_of_nodup H.nodup_names] at h₁
+    simp at h₁
+    choose d' h₁ using h₁
+    have h₃ := H.nodup_names
+    rw [List.nodup_map_iff_inj_on # List.Nodup.of_map _ h₃] at h₃
+    rw [List.find?_eq_some_iff_of_at_most_one] at h₁; grind
+    rintro ⟨name₁, d₁⟩ ⟨name₂, d₂⟩ h₄ h₅
+    simp
+    rintro rfl rfl
+    simp
+    grind
+  · exact H.compatible_fs
+
+theorem wf_of_wfDefs {defs} (H : WFDefs defs) : (Prog.ofDefs defs).WF := H.wf
+
 @[simp, instance]
 theorem wf_progId : progId.WF := by
-  constructor <;> try simp [exprId]
-  use [fn 1 λ xs => xs[0]!]; unfold fn
-  simp; split_ands; constructor <;> simp [exprId] <;> grind
-  rintro fs ⟨h₁, h₂, h₃⟩; simp at h₁ h₂ h₃
-  rw [List.length_eq_one_iff] at h₁; simp [exprId] at h₃
-  obtain ⟨f, rfl⟩ := h₁; simp at h₂ h₃ ⊢; grind
+  apply wf_of_wfDefs
+  constructor <;> try simp
+  use .ofList [(mainName, fn 1 λ xs => xs[0]!)]
+  split_ands
+  ·
+    dsimp
+    constructor
+    ·
+      simp
+
+#check 0 #exit
 
 @[simp]
 theorem Expr.run_call {prog fs args t xs} : (Expr.call t xs).eval prog fs args =
