Projects/Esolangs/Cornucopia/Defs.lean
@@ -1,20 +1,93 @@
 import Projects.Util
 
+def mkList {α : Type*} (n : ℕ) (f : ℕ → α) : List α :=
+  List.range n |>.map f
+
+instance : LinearOrder String where
+  le_refl := by grind
+  le_trans := by grind
+  le_antisymm := by grind
+  le_total := by grind
+  toDecidableLE := inferInstance
+  lt_iff_le_not_ge := by grind
+  min_def := by
+    intro a b; change ite _ _ _ = _; congr
+    change (Ordering.isLE (ite _ _ _) = _) = _
+    have h : (a < b) = ¬(b ≤ a); change _ = ¬¬_; simp
+    simp [apply_ite (f := Ordering.isLE)]; grind
+  max_def := by
+    intro a b; change ite _ _ _ = _; congr
+    change (Ordering.isLE (ite _ _ _) = _) = _
+    have h : (a < b) = ¬(b ≤ a); change _ = ¬¬_; simp
+    simp [apply_ite (f := Ordering.isLE)]; grind
+  compare_eq_compareOfLessAndEq := by
+    intro a b; change compareOfLessAndEq _ _ = _; congr
+
+-- namespace List
+-- 
+-- variable {α β γ : Type*}
+-- variable {xs ys zs : List α}
+-- 
+-- -- #check 0 #exit
+-- 
+-- end List
+
+-- #check 0 #exit
+
+namespace Finset
+
+variable {α β γ : Type*}
+variable {s s₁ s₂ s₃ : Finset α}
+
+def fold' (s : Finset α) (f : β → α → β) (z : β)
+(h : ∀ {acc x y}, f (f acc x) y = f (f acc y) x) : β :=
+  haveI : RightCommutative f := ⟨@h⟩; s.val.foldl f z
+
+-- #check 0 #exit
+
+end Finset
+
+-- namespace Map
+-- 
+-- open Std
+-- 
+-- universe u v w
+-- variable {α : Type u} {β : Type v} {γ : Type w}
+-- variable [hh₁ : DecidableEq α] [hh₂ : Hashable α]
+-- variable {mp : Map α β}
+-- variable [ha : LinearOrder α]
+-- omit ha
+-- 
+-- def ofFinset (s : Finset (α × β)) : Map α β :=
+--   s.fold' (z := ∅) (λ m ⟨k, v⟩ => m.insert k v) #
+--     by
+--       intro m x y
+--       simp
+--       rw [insert_comm]
+-- 
+-- #check 0 #exit
+-- 
+-- end Map
+
 namespace Esolangs.Cornucopia
+
+def mainName : String := "main"
 
 inductive Builtin : Type where
 | succ : Builtin
 | sub : Builtin
 deriving Inhabited, Fintype, DecidableEq
 
-inductive Target : Type where
-| builtin : Builtin → Target
-| custom : ℕ → Target
-deriving Inhabited, DecidableEq
+@[ext]
+structure BuiltinInfo : Type where
+  name : String
+  arity : ℕ
+  eval : List ℕ → ℕ
+deriving Inhabited
 
 inductive Expr : Type where
 | arg : ℕ → Expr
-| call : Target → List Expr → Expr
+| call : String → List Expr → Expr
 deriving Inhabited
 
 @[ext]
@@ -25,119 +98,123 @@ deriving Inhabited
 
 @[ext]
 structure Prog : Type where
-  defs : List Def
+  defs : Map String Def
 deriving Inhabited
 
 -----
 
-def Prog.def (prog : Prog) (i : ℕ) : Def :=
-  prog.defs[i]!
+-- #check 0 #exit
+
+def fn (arity : ℕ) (f : List ℕ → ℕ) (xs : List ℕ) : ℕ :=
+  if xs.length ≠ arity then 0 else f xs
+
+def builtins : List Builtin :=
+  [.succ, .sub]
+
+def Builtin.info (b : Builtin) : BuiltinInfo :=
+  match b with
+  | .succ => {name := "succ", arity := 1, eval xs := xs[0]! + 1}
+  | .sub => {name := "sub", arity := 2, eval xs := xs[0]! - xs[1]!}
+
+def Builtin.name (b : Builtin) : String := b.info.name
+def Builtin.arity (b : Builtin) : ℕ := b.info.arity
+def Builtin.eval (b : Builtin) : List ℕ → ℕ := fn b.arity b.info.eval
+
+def Builtin.expr (b : Builtin) : Expr :=
+  .call b.name # mkList b.arity .arg
+
+def Builtin.def (b : Builtin) : Def where
+  arity := b.arity
+  expr := b.expr
+
+def Builtin.namesMap : Map String Builtin :=
+  .ofList # builtins.map λ b => (b.name, b)
+
+def IsBuiltin (name : String) : Prop :=
+  ∃ (b : Builtin), b.name = name
+
+def Prog.def? (prog : Prog) (name : String) : Option Def :=
+  prog.defs.get? name
+
+def Prog.def (prog : Prog) (name : String) : Def :=
+  prog.defs.get! name
+
+def builtinDefs : Map String Def :=
+  .ofList # builtins.map (λ b => (b.name, b.def))
+
+def builtinFs : Map String (List ℕ → ℕ) :=
+  .ofList # builtins.map (λ b => (b.name, b.eval))
+
+def Prog.ofDefs (defs : List (String × Def)) : Prog where
+  defs := builtinDefs ∪ .ofList defs
 
 def Prog.main (prog : Prog) : Def :=
-  prog.def 0
+  prog.def mainName
 
-def Prog.HasDef (prog : Prog) (i : ℕ) : Prop :=
-  i < prog.defs.length
+def Prog.HasDef (prog : Prog) (name : String) : Prop :=
+  name ∈ prog.defs
 
-def Prog.arity (prog : Prog) (i : ℕ) : ℕ :=
-  prog.def i |>.arity
+def Prog.arity (prog : Prog) (name : String) : ℕ :=
+  prog.def name |>.arity
 
-def Prog.expr (prog : Prog) (i : ℕ) : Expr :=
-  prog.def i |>.expr
-
-def Builtin.arity (bn : Builtin) : ℕ :=
-  match bn with
-  | .succ => 1
-  | .sub => 2
-
-def Target.arity (t : Target) (prog : Prog) : ℕ :=
-  match t with
-  | .builtin bn => bn.arity
-  | .custom i => prog.arity i
-
-def Prog.HasTarget (prog : Prog) (t : Target) : Prop :=
-  match t with
-  | .builtin _ => True
-  | .custom i => prog.HasDef i
+def Prog.expr (prog : Prog) (name : String) : Expr :=
+  prog.def name |>.expr
 
 def Expr.WF (prog : Prog) (arity : ℕ) (e : Expr) : Prop :=
   match e with
   | .arg i => i < arity
-  | .call t args => prog.HasTarget t ∧ args.length = t.arity prog ∧
+  | .call t args => prog.HasDef t ∧ args.length = prog.arity t ∧
     ∀ e ∈ args, e.WF prog arity
 
 @[simp]
 def Def.WF (prog : Prog) (d : Def) : Prop :=
   d.expr.WF prog d.arity
 
-def Builtin.f (bn : Builtin) (args : List ℕ) : ℕ :=
-  match bn with
-  | .succ => args[0]! + 1
-  | .sub => args[0]! - args[1]!
-
-def Target.f (t : Target) (fs : List (List ℕ → ℕ)) : List ℕ → ℕ :=
-  match t with
-  | .builtin bn => bn.f
-  | .custom i => fs[i]!
-
-def Expr.eval (e : Expr) (prog : Prog) (fs : List (List ℕ → ℕ)) (args : List ℕ) : ℕ :=
+def Expr.eval (e : Expr) (prog : Prog) (fs : Map String (List ℕ → ℕ)) (args : List ℕ) : ℕ :=
   match e with
   | .arg i => args[i]!
-  | .call t xs => t.f fs # xs.map λ x => x.eval prog fs args
+  | .call t xs => fs.get! t # xs.map λ x => x.eval prog fs args
 
-structure Prog.Compatible (prog : Prog) (fs : List (List ℕ → ℕ)) : Prop where
-  length_fs : fs.length = prog.defs.length
-  eq_default_of_ne_arity ⦃i⦄ : i < prog.defs.length → ∀ ⦃xs : List ℕ⦄,
-    xs.length ≠ prog.arity i → fs[i]! xs = default
-  eval_eq ⦃i⦄ : i < prog.defs.length → ∀ ⦃xs : List ℕ⦄, xs.length = prog.arity i →
-    fs[i]! xs = (prog.expr i).eval prog fs xs
+structure Prog.Compatible (prog : Prog) (fs : Map String (List ℕ → ℕ)) : Prop where
+  keys_fs : fs.keys = prog.defs.keys
+  eval_of_ne_arity ⦃name⦄ : prog.HasDef name → ∀ ⦃xs : List ℕ⦄,
+    xs.length ≠ prog.arity name → fs.get! name xs = 0
+  eval_eq ⦃name⦄ : prog.HasDef name → ∀ ⦃xs : List ℕ⦄, xs.length = prog.arity name →
+    fs.get! name xs = (prog.expr name).eval prog fs xs
 
 class Prog.WF (prog : Prog) : Prop where
-  defs_ne_nil : prog.defs ≠ []
+  def?_builtin {b : Builtin} : prog.def? b.name = some b.def
+  has_main : prog.HasDef mainName
   arity_main : prog.main.arity = 1
-  wf_def ⦃d⦄ : d ∈ prog.defs → d.WF prog
+  wf_def ⦃name d⦄ : prog.def? name = some d → d.WF prog
   exiu_compatible : ∃! fs, prog.Compatible fs
 
-open Classical in noncomputable
-def Prog.fs (prog : Prog) : List (List ℕ → ℕ) :=
+in noncomputable
+def Prog.fs (prog : Prog) : Map String (List ℕ → ℕ) :=
   τ fs, prog.Compatible fs
 
-open Classical in noncomputable
-def Prog.eval (prog : Prog) (i : ℕ) (xs : List ℕ) : ℕ :=
-  prog.fs[i]! xs
+in noncomputable
+def Prog.eval (prog : Prog) (name : String) (xs : List ℕ) : ℕ :=
+  prog.fs.get! name xs
 
-open Classical in noncomputable
+in noncomputable
 def Prog.run (prog : Prog) (n : ℕ) : ℕ :=
-  prog.eval 0 [n]
+  prog.eval mainName [n]
 
-def fn (arity : ℕ) (f : List ℕ → ℕ) (xs : List ℕ) : ℕ :=
-  if xs.length ≠ arity then default else f xs
-
-def Builtin.show (b : Builtin) : String :=
-  match b with
-  | .succ => "succ"
-  | .sub => "sub"
-
-def Target.show (t : Target) (defNames : Array String) : String :=
-  match t with
-  | .builtin b => b.show
-  | .custom i => defNames[i - 1]!
-
-def Expr.show (e : Expr) (defNames argNames : Array String) : String :=
+def Expr.show (e : Expr) (argNames : Array String) : String :=
   match e with
   | .arg i => argNames[i]!
   | .call t args =>
-    t.show defNames ++ if args.length = 0 then "" else
-      "(" ++ ", ".intercalate (args.map (·.show defNames argNames)) ++ ")"
+    t ++ if args.length = 0 then "" else
+    "(" ++ ", ".intercalate (args.map (·.show argNames)) ++ ")"
 
-def Def.show (d : Def) (defNames : Array String) (name : String) : String :=
-  let argNames := List.range d.arity |>.map λ i => String.ofList [.ofNat # 97 + i]
-  name ++ "".intercalate (argNames.map (" " ++ ·)) ++ " := " ++
-    d.expr.show defNames ⟨argNames⟩
+def Def.show (d : Def) (name : String) : String :=
+  let argNamesList := mkList d.arity λ i => String.ofList [.ofNat # 97 + i]
+  let argNames := .mk argNamesList
+  let argsStr := if d.arity = 0 then "" else
+    "(" ++ "".intercalate (argNamesList.map (", " ++ ·)) ++ ")"
+  name ++ argsStr ++ " := " ++ d.expr.show argNames
 
-def Prog.show (prog : Prog) (defNames : Array String) : String :=
-  match prog.defs with
-  | mainDef :: defs =>
-    let xs := defs.zipWith (Def.show · defNames) defNames.toList
-    "\n".intercalate # xs ++ [mainDef.show defNames "main"]
-  | _ => ""
+def Prog.show (prog : Prog) (defNames : List String) : String :=
+  if ¬defNames.Perm prog.defs.keys then "/" else
+  "\n".intercalate # defNames.map # λ name => prog.def name |>.show name
